Logic/FoundationPort/Coq/FirstOrder/Arithmetic/R0/Basic.v
@@ -7,12 +7,154 @@
   retaining the exact numeral arithmetic and finite-interval content.
 *)
 
-From Stdlib Require Import Arith.PeanoNat Lia Vectors.Fin.
-From Foundation.FirstOrder.Arithmetic.Basic Require Import Misc.
+From Stdlib Require Import Arith.PeanoNat Lia Logic.Classical_Prop Vectors.Fin.
+From FoundationModal Require Import GenericAdjunctiveSet GenericEntailment.
+From Foundation.Syntax.Predicate Require Import Language Quantifier Term.
+From Foundation.FirstOrder.Basic.Syntax Require Import Formula.
+From Foundation.FirstOrder.Basic Require Import Calculus Eq Operator Soundness.
+From Foundation.FirstOrder.Basic.Semantics Require Import
+  ModelTheory RewriteClosure Semantics OperatorSemantics.
+From Foundation.FirstOrder.Arithmetic.Basic Require Import Misc Syntax Model.
 
 Set Implicit Arguments.
 Unset Strict Implicit.
 Set Universe Polymorphism.
+
+(** * The concrete Cobham-R0 theory *)
+
+Definition r0_numeral_add_sentence (n m : nat) : sentence oring_language :=
+  arithmetic_eq_formula
+    (arithmetic_add_term (arithmetic_numeral_term n)
+      (arithmetic_numeral_term m))
+    (arithmetic_numeral_term (n + m)).
+
+Definition r0_numeral_mul_sentence (n m : nat) : sentence oring_language :=
+  arithmetic_eq_formula
+    (arithmetic_mul_term (arithmetic_numeral_term n)
+      (arithmetic_numeral_term m))
+    (arithmetic_numeral_term (n * m)).
+
+Definition r0_numeral_ne_sentence (n m : nat) : sentence oring_language :=
+  semiformula_neg
+    (arithmetic_eq_formula (arithmetic_numeral_term n)
+      (arithmetic_numeral_term m)).
+
+Definition r0_initial_segment_sentence (n : nat) : sentence oring_language :=
+  first_all_closure
+    (semiformula_universal_quantifier oring_language Empty_set) 1
+    (semiformula_iff
+      (arithmetic_lt_formula
+        (@Semiterm_bvar oring_language Empty_set 1 Fin.F1)
+        (arithmetic_numeral_term n))
+      (arithmetic_eq_disjunction n
+        (@Semiterm_bvar oring_language Empty_set 1 Fin.F1))).
+
+Inductive r0_axiom : theory oring_language :=
+| R0Equality : forall sigma,
+    first_order_equality_axiom oring_language_eq_operator sigma ->
+    r0_axiom sigma
+| R0NumeralAdd : forall n m,
+    r0_axiom (r0_numeral_add_sentence n m)
+| R0NumeralMul : forall n m,
+    r0_axiom (r0_numeral_mul_sentence n m)
+| R0NumeralNe : forall n m,
+    n <> m -> r0_axiom (r0_numeral_ne_sentence n m)
+| R0InitialSegment : forall n,
+    r0_axiom (r0_initial_segment_sentence n).
+
+Theorem r0_proves_equality :
+  first_order_theory_proves_equality r0_axiom oring_language_eq_operator.
+Proof.
+  intros sigma Hsigma.
+  exact (@generic_axiomatized_by_axiom
+    (theory oring_language) (sentence oring_language)
+    (first_order_theory_entailment oring_language)
+    (generic_predicate_adjunctive_set (sentence oring_language))
+    (first_order_theory_axiomatized oring_language)
+    r0_axiom sigma (R0Equality Hsigma)).
+Qed.
+
+Definition r0_empty_bound_env : Fin.t 0 -> nat :=
+  fun i => match i with end.
+
+Definition r0_empty_free_env {A} : Empty_set -> A :=
+  fun x => match x with end.
+
+Lemma r0_numeral_add_realize_iff : forall M
+    (Str : first_order_structure oring_language M) (O : oring_carrier M) n m,
+  structure_interprets_oring Str oring_language_structure O ->
+  (sentence_realize Str (r0_numeral_add_sentence n m) <->
+   oring_add O (oring_numeral O n) (oring_numeral O m) =
+   oring_numeral O (n + m)).
+Proof.
+  intros M Str O n m Horing. unfold sentence_realize,
+    r0_numeral_add_sentence, formula_eval.
+  rewrite (@arithmetic_eq_formula_eval M Empty_set 0 Str _ _ O _ _ Horing).
+  rewrite (@arithmetic_add_term_val M Empty_set 0 Str _ _ O _ _ Horing).
+  repeat rewrite (@arithmetic_numeral_term_val M Empty_set 0 Str _ _ O _ Horing).
+  reflexivity.
+Qed.
+
+Lemma r0_numeral_mul_realize_iff : forall M
+    (Str : first_order_structure oring_language M) (O : oring_carrier M) n m,
+  structure_interprets_oring Str oring_language_structure O ->
+  (sentence_realize Str (r0_numeral_mul_sentence n m) <->
+   oring_mul O (oring_numeral O n) (oring_numeral O m) =
+   oring_numeral O (n * m)).
+Proof.
+  intros M Str O n m Horing. unfold sentence_realize,
+    r0_numeral_mul_sentence, formula_eval.
+  rewrite (@arithmetic_eq_formula_eval M Empty_set 0 Str _ _ O _ _ Horing).
+  rewrite (@arithmetic_mul_term_val M Empty_set 0 Str _ _ O _ _ Horing).
+  repeat rewrite (@arithmetic_numeral_term_val M Empty_set 0 Str _ _ O _ Horing).
+  reflexivity.
+Qed.
+
+Lemma r0_numeral_ne_realize_iff : forall M
+    (Str : first_order_structure oring_language M) (O : oring_carrier M) n m,
+  structure_interprets_oring Str oring_language_structure O ->
+  (sentence_realize Str (r0_numeral_ne_sentence n m) <->
+   oring_numeral O n <> oring_numeral O m).
+Proof.
+  intros M Str O n m Horing. unfold sentence_realize,
+    r0_numeral_ne_sentence, formula_eval.
+  rewrite semiformula_eval_neg.
+  rewrite (@arithmetic_eq_formula_eval M Empty_set 0 Str _ _ O _ _ Horing).
+  repeat rewrite (@arithmetic_numeral_term_val M Empty_set 0 Str _ _ O _ Horing).
+  reflexivity.
+Qed.
+
+Lemma r0_initial_segment_realize_iff : forall M
+    (Str : first_order_structure oring_language M) (O : oring_carrier M) n,
+  structure_interprets_oring Str oring_language_structure O ->
+  (sentence_realize Str (r0_initial_segment_sentence n) <->
+   forall x,
+     oring_lt O x (oring_numeral O n) <->
+     exists i : Fin.t n,
+       x = oring_numeral O (proj1_sig (Fin.to_nat i))).
+Proof.
+  intros M Str O n Horing. unfold sentence_realize,
+    r0_initial_segment_sentence, formula_eval.
+  rewrite semiformula_eval_all_closure. split.
+  - intros H x. specialize (H (fin_one x)).
+    rewrite semiformula_eval_iff in H.
+    rewrite (@arithmetic_lt_formula_eval M Empty_set 1 Str (fin_one x)
+      r0_empty_free_env O _ _ Horing) in H.
+    rewrite (@arithmetic_numeral_term_val M Empty_set 1 Str (fin_one x)
+      r0_empty_free_env O _ Horing) in H.
+    rewrite (@arithmetic_eq_disjunction_eval M Empty_set 1 Str (fin_one x)
+      r0_empty_free_env O n _ Horing) in H.
+    simpl in H. exact H.
+  - intros H e. specialize (H (e Fin.F1)).
+    rewrite semiformula_eval_iff.
+    rewrite (@arithmetic_lt_formula_eval M Empty_set 1 Str e
+      r0_empty_free_env O _ _ Horing).
+    rewrite (@arithmetic_numeral_term_val M Empty_set 1 Str e
+      r0_empty_free_env O _ Horing).
+    rewrite (@arithmetic_eq_disjunction_eval M Empty_set 1 Str e
+      r0_empty_free_env O n _ Horing).
+    simpl. exact H.
+Qed.
 
 Record r0_laws {M : Type} (O : oring_carrier M) : Prop := {
   r0_numeral_add : forall n m,
@@ -68,6 +210,54 @@ Proof.
     + exact Hx.
 Qed.
 
+Theorem first_order_model_models_r0_iff : forall
+    (m : first_order_model oring_language)
+    (O : oring_carrier (first_order_model_domain m)),
+  structure_interprets_oring (first_order_model_structure m)
+    oring_language_structure O ->
+  (first_order_models_theory m r0_axiom <-> r0_laws O).
+Proof.
+  intros m O Horing. split.
+  - intro Hmodels. constructor.
+    + intros n q. apply (proj1 (@r0_numeral_add_realize_iff _
+        (first_order_model_structure m) O n q Horing)).
+      exact (first_order_models_of_member Hmodels (R0NumeralAdd n q)).
+    + intros n q. apply (proj1 (@r0_numeral_mul_realize_iff _
+        (first_order_model_structure m) O n q Horing)).
+      exact (first_order_models_of_member Hmodels (R0NumeralMul n q)).
+    + intros n q Hne. apply (proj1 (@r0_numeral_ne_realize_iff _
+        (first_order_model_structure m) O n q Horing)).
+      exact (first_order_models_of_member Hmodels (R0NumeralNe Hne)).
+    + intros n x.
+      pose proof (proj1 (@r0_initial_segment_realize_iff _
+        (first_order_model_structure m) O n Horing)
+        (first_order_models_of_member Hmodels (R0InitialSegment n))) as Hfin.
+      specialize (Hfin x). split.
+      * intro Hx. destruct (proj1 Hfin Hx) as [i Hi].
+        exists (proj1_sig (Fin.to_nat i)). split.
+        -- exact (proj2_sig (Fin.to_nat i)).
+        -- exact Hi.
+      * intros [i [Hin Hi]]. apply (proj2 Hfin).
+        exists (Fin.of_nat_lt Hin). rewrite Fin.to_nat_of_nat. exact Hi.
+  - intro Hlaws. apply (proj2 (first_order_models_theory_iff m _)).
+    intros sigma Hsigma. destruct Hsigma.
+    + exact (first_order_models_of_member
+        (first_order_model_models_equality_theory_of_interprets_eq
+          (structure_oring_eq Horing)) H).
+    + apply (proj2 (@r0_numeral_add_realize_iff _
+        (first_order_model_structure m) O n m0 Horing)).
+      exact (r0_numeral_add Hlaws n m0).
+    + apply (proj2 (@r0_numeral_mul_realize_iff _
+        (first_order_model_structure m) O n m0 Horing)).
+      exact (r0_numeral_mul Hlaws n m0).
+    + apply (proj2 (@r0_numeral_ne_realize_iff _
+        (first_order_model_structure m) O n m0 Horing)).
+      exact (r0_numeral_ne Hlaws H).
+    + apply (proj2 (@r0_initial_segment_realize_iff _
+        (first_order_model_structure m) O n Horing)).
+      intros x. exact (r0_lt_numeral_fin_iff Hlaws n x).
+Qed.
+
 Definition nat_r0_laws : r0_laws nat_oring_carrier.
 Proof.
   constructor.
@@ -82,3 +272,118 @@ Proof.
     + intros [i [Hin ->]]. rewrite nat_oring_numeral.
       change (i < n). exact Hin.
 Defined.
+
+Theorem nat_standard_model_models_r0 :
+  first_order_models_theory nat_standard_model r0_axiom.
+Proof.
+  apply (proj2 (@first_order_model_models_r0_iff
+    nat_standard_model nat_oring_carrier nat_standard_structure_interprets)).
+  exact nat_r0_laws.
+Qed.
+
+Theorem r0_consistent :
+  generic_consistent (first_order_theory_entailment oring_language) r0_axiom.
+Proof.
+  exact (first_order_theory_consistent_of_model nat_standard_model_models_r0).
+Qed.
+
+Theorem r0_proof_complete : forall sigma : sentence oring_language,
+  (forall (m : first_order_model oring_language)
+          (O : oring_carrier (first_order_model_domain m)),
+    structure_interprets_oring (first_order_model_structure m)
+      oring_language_structure O ->
+    r0_laws O ->
+    first_order_model_realize m sigma) ->
+  first_order_theory_provable r0_axiom sigma.
+Proof.
+  intros sigma Hvalid.
+  apply (arithmetic_theory_proof_complete r0_proves_equality).
+  intros m O Horing Hmodels.
+  apply (Hvalid m O Horing).
+  now apply (proj1 (@first_order_model_models_r0_iff m O Horing)).
+Qed.
+
+(** The source's omega-plus-one R0 countermodel.  Unlike the Q countermodel
+    used elsewhere, every operation involving the extra top point collapses
+    to zero; hence [top + 0 <> top]. *)
+Definition r0_omega_add_one : Type := option nat.
+
+Definition r0_omega_add_one_add
+    (x y : r0_omega_add_one) : r0_omega_add_one :=
+  match x, y with
+  | Some n, Some m => Some (n + m)
+  | _, _ => Some 0
+  end.
+
+Definition r0_omega_add_one_mul
+    (x y : r0_omega_add_one) : r0_omega_add_one :=
+  match x, y with
+  | Some n, Some m => Some (n * m)
+  | _, _ => Some 0
+  end.
+
+Definition r0_omega_add_one_lt
+    (x y : r0_omega_add_one) : Prop :=
+  match x, y with
+  | Some n, Some m => n < m
+  | Some _, None => True
+  | None, _ => False
+  end.
+
+Definition r0_omega_add_one_oring : oring_carrier r0_omega_add_one :=
+  {| oring_zero := Some 0;
+     oring_one := Some 1;
+     oring_add := r0_omega_add_one_add;
+     oring_mul := r0_omega_add_one_mul;
+     oring_lt := r0_omega_add_one_lt |}.
+
+Lemma r0_omega_add_one_numeral : forall n,
+  oring_numeral r0_omega_add_one_oring n = Some n.
+Proof.
+  induction n as [|n IH]; [reflexivity|].
+  destruct n as [|n]; [reflexivity|].
+  change (r0_omega_add_one_add
+    (oring_numeral r0_omega_add_one_oring (S n)) (Some 1) =
+    Some (S (S n))).
+  rewrite IH. cbn [r0_omega_add_one_add]. f_equal. lia.
+Qed.
+
+Definition r0_omega_add_one_laws : r0_laws r0_omega_add_one_oring.
+Proof.
+  constructor.
+  - intros n m. rewrite !r0_omega_add_one_numeral.
+    cbv [r0_omega_add_one_oring r0_omega_add_one_add oring_add]. f_equal.
+  - intros n m. rewrite !r0_omega_add_one_numeral.
+    cbv [r0_omega_add_one_oring r0_omega_add_one_mul oring_mul]. f_equal.
+  - intros n m Hne. rewrite !r0_omega_add_one_numeral.
+    intro Heq. injection Heq. contradiction.
+  - intros n [x|].
+    + rewrite r0_omega_add_one_numeral.
+      cbv [r0_omega_add_one_oring r0_omega_add_one_lt oring_lt]. split.
+      * intro Hx. exists x. split; [exact Hx|].
+        symmetry. apply r0_omega_add_one_numeral.
+      * intros [i [Hin Hi]]. rewrite r0_omega_add_one_numeral in Hi.
+        injection Hi. intro Hxi. subst i. exact Hin.
+    + rewrite r0_omega_add_one_numeral.
+      cbv [r0_omega_add_one_oring r0_omega_add_one_lt oring_lt]. split.
+      * contradiction.
+      * intros [i [Hin Hi]]. rewrite r0_omega_add_one_numeral in Hi.
+        discriminate.
+Defined.
+
+Definition r0_omega_add_one_model : first_order_model oring_language :=
+  first_order_model_of_structure (inhabits None)
+    (oring_standard_structure r0_omega_add_one_oring).
+
+Theorem r0_omega_add_one_model_models_r0 :
+  first_order_models_theory r0_omega_add_one_model r0_axiom.
+Proof.
+  apply (proj2 (@first_order_model_models_r0_iff
+    r0_omega_add_one_model r0_omega_add_one_oring
+    (oring_standard_structure_interprets r0_omega_add_one_oring))).
+  exact r0_omega_add_one_laws.
+Qed.
+
+Lemma r0_omega_add_one_top_add_zero :
+  r0_omega_add_one_add None (oring_zero r0_omega_add_one_oring) = Some 0.
+Proof. reflexivity. Qed.
